Tidied up a bit more

inference-tool/src/main/scala/inference/Inference.scala
@@ -707,6 +707,14 @@ def map[A, B](f: A => B, l: List[A]): List[B] = l.par.map(f).toList
 def product[A, B](xs: List[A], ys: List[B]): List[(A, B)] =
   maps[A, (A, B)](((x: A) => map[B, (A, B)](((a: B) => (x, a)), ys)), xs)
 
+def subseqs[A](x0: List[A]): List[List[A]] = x0 match {
+  case Nil => List(Nil)
+  case x :: xs => {
+                    val xss: List[List[A]] = subseqs[A](xs);
+                    map[List[A], List[A]](((a: List[A]) => x :: a), xss) ++ xss
+                  }
+}
+
 def enumerate[A](n: Nat.nat, xs: List[A]): List[(Nat.nat, A)] =
   (upt(n, Nat.plus_nata(n, Nat.Nata(xs.par.length)))).par.zip(xs).toList
 
@@ -734,6 +742,16 @@ def list_update[A](x0: List[A], i: Nat.nat, y: A): List[A] = (x0, i, y) match {
   case (x :: xs, i, y) =>
     (if (Nat.equal_nata(i, Nat.zero_nata)) y :: xs
       else x :: list_update[A](xs, Nat.minus_nat(i, Nat.Nata((1))), y))
+}
+
+def product_lists[A](x0: List[List[A]]): List[List[A]] = x0 match {
+  case Nil => List(Nil)
+  case xs :: xss =>
+    maps[A, List[A]](((x: A) =>
+                       map[List[A],
+                            List[A]](((a: List[A]) => x :: a),
+                                      product_lists[A](xss))),
+                      xs)
 }
 
 def insort_key[A, B : Orderings.linorder](f: A => B, x: A, xa2: List[A]):
@@ -785,47 +803,37 @@ object Set {
 abstract sealed class set[A]
 final case class seta[A](a: List[A]) extends set[A]
 
-def insert[A](x: A, xa1: set[A]): set[A] = (x, xa1) match {
-  case (x, seta(s)) => (if (s.contains(x)) seta[A](s) else seta[A](x :: s))
+def Ball[A](x0: set[A], p: A => Boolean): Boolean = (x0, p) match {
+  case (seta(xs), p) => Lista.list_all[A](p, xs)
 }
-
-def sup_set[A](x0: set[A], a: set[A]): set[A] = (x0, a) match {
-  case (seta(x), seta(y)) => seta[A](x ++ y)
-  case (seta(xs), a) =>
-    Lista.fold[A, set[A]](((aa: A) => (b: set[A]) => insert[A](aa, b)), xs, a)
-}
-
-def bot_set[A]: set[A] = seta[A](Nil)
 
 def image[A, B](f: A => B, x1: set[A]): set[B] = (f, x1) match {
   case (f, seta(xs)) => seta[B](Lista.map[A, B](f, xs))
-}
-
-def Pow[A](x0: set[A]): set[set[A]] = x0 match {
-  case seta(x :: xs) =>
-    {
-      val a: set[set[A]] = Pow[A](seta[A](xs));
-      sup_set[set[A]](a, image[set[A],
-                                set[A]](((aa: set[A]) => insert[A](x, aa)), a))
-    }
-  case seta(Nil) => insert[set[A]](bot_set[A], bot_set[set[A]])
-}
-
-def Ball[A](x0: set[A], p: A => Boolean): Boolean = (x0, p) match {
-  case (seta(xs), p) => Lista.list_all[A](p, xs)
 }
 
 def filter[A](p: A => Boolean, x1: set[A]): set[A] = (p, x1) match {
   case (p, seta(xs)) => seta[A](Lista.filter[A](p, xs))
 }
 
+def insert[A](x: A, xa1: set[A]): set[A] = (x, xa1) match {
+  case (x, seta(s)) => (if (s.contains(x)) seta[A](s) else seta[A](x :: s))
+}
+
 def member[A](x: A, xa1: set[A]): Boolean = (x, xa1) match {
   case (x, seta(xs)) => xs.contains(x)
 }
 
+def bot_set[A]: set[A] = seta[A](Nil)
+
 def inf_set[A](a: set[A], x1: set[A]): set[A] = (a, x1) match {
   case (a, seta(xs)) =>
     seta[A](Lista.filter[A](((x: A) => member[A](x, a)), xs))
+}
+
+def sup_set[A](x0: set[A], a: set[A]): set[A] = (x0, a) match {
+  case (seta(x), seta(y)) => seta[A](x ++ y)
+  case (seta(xs), a) =>
+    Lista.fold[A, set[A]](((aa: A) => (b: set[A]) => insert[A](aa, b)), xs, a)
 }
 
 def less_eq_set[A](a: set[A], b: set[A]): Boolean =
@@ -6557,6 +6565,29 @@ def target(tRegs: Map[Nat.nat, Option[Value.value]],
                Map[Nat.nat, Option[Value.value]], List[Value.value],
                List[Nat.nat], Transition.transition_ext[Unit]](tRegs, ts, Nil)
 
+def unzip_3_tailrec_rev[A, B,
+                         C](x0: List[(A, (B, C))],
+                             x1: (List[A], (List[B], List[C]))):
+      (List[A], (List[B], List[C]))
+  =
+  (x0, x1) match {
+  case (Nil, (as, (bs, cs))) => (as, (bs, cs))
+  case ((a, (b, c)) :: t, (as, (bs, cs))) =>
+    unzip_3_tailrec_rev[A, B, C](t, (a :: as, (b :: bs, c :: cs)))
+}
+
+def unzip_3_tailrec[A, B, C](l: List[(A, (B, C))]):
+      (List[A], (List[B], List[C]))
+  =
+  {
+    val (as, (bs, cs)): (List[A], (List[B], List[C])) =
+      unzip_3_tailrec_rev[A, B, C](l, (Nil, (Nil, Nil)));
+    (as.par.reverse.toList, (bs.par.reverse.toList, cs.par.reverse.toList))
+  }
+
+def unzip_3[A, B, C](l: List[(A, (B, C))]): (List[A], (List[B], List[C])) =
+  unzip_3_tailrec[A, B, C](l)
+
 def group_by[A](uu: A => A => Boolean, x1: List[A]): List[List[A]] = (uu, x1)
   match {
   case (uu, Nil) => Nil
@@ -6571,15 +6602,6 @@ def group_by[A](uu: A => A => Boolean, x1: List[A]): List[List[A]] = (uu, x1)
           })
      })
 }
-
-def cartProdN[A](l: List[List[A]]): List[List[A]] =
-  Lista.foldr[List[A],
-               List[List[A]]](((xs: List[A]) => (as: List[List[A]]) =>
-                                Lista.maps[A,
-    List[A]](((x: A) =>
-               Lista.map[List[A], List[A]](((a: List[A]) => x :: a), as)),
-              xs)),
-                               l, List(Nil))
 
 def replace_transition(e: FSet.fset[(List[Nat.nat],
                                       ((Nat.nat, Nat.nat),
@@ -6616,6 +6638,213 @@ Transition.transition_ext[Unit]))],
                 }),
                e)
 
+def find_outputs(x0: List[List[AExp.aexp[VName.vname]]],
+                  uu: FSet.fset[(List[Nat.nat],
+                                  ((Nat.nat, Nat.nat),
+                                    Transition.transition_ext[Unit]))],
+                  uv: List[List[(String,
+                                  (List[Value.value], List[Value.value]))]],
+                  uw: List[(List[Nat.nat], Transition.transition_ext[Unit])]):
+      Option[List[AExp.aexp[VName.vname]]]
+  =
+  (x0, uu, uv, uw) match {
+  case (Nil, uu, uv, uw) => None
+  case (h :: t, e, l, g) =>
+    {
+      val outputs:
+            FSet.fset[(List[Nat.nat],
+                        ((Nat.nat, Nat.nat), Transition.transition_ext[Unit]))]
+        = Lista.fold[(List[Nat.nat], Transition.transition_ext[Unit]),
+                      FSet.fset[(List[Nat.nat],
+                                  ((Nat.nat, Nat.nat),
+                                    Transition.transition_ext[Unit]))]](((a:
+                                    (List[Nat.nat],
+                                      Transition.transition_ext[Unit]))
+                                   =>
+                                  {
+                                    val (tids, ta):
+  (List[Nat.nat], Transition.transition_ext[Unit])
+                                      = a;
+                                    ((acc:
+FSet.fset[(List[Nat.nat],
+            ((Nat.nat, Nat.nat), Transition.transition_ext[Unit]))])
+                                       =>
+                                      replace_transition(acc, tids,
+                  Transition.Outputs_update[Unit](((_:
+              List[AExp.aexp[VName.vname]])
+             =>
+            h),
+           ta)))
+                                  }),
+                                 g, e);
+      (if (Inference.satisfies(Set.seta[List[(String,
+       (List[Value.value], List[Value.value]))]](l),
+                                Inference.tm(outputs)))
+        Some[List[AExp.aexp[VName.vname]]](h) else find_outputs(t, e, l, g))
+    }
+}
+
+def find_updates_outputs(x0: List[List[(Nat.nat, AExp.aexp[VName.vname])]],
+                          uu: List[List[AExp.aexp[VName.vname]]],
+                          uv: FSet.fset[(List[Nat.nat],
+  ((Nat.nat, Nat.nat), Transition.transition_ext[Unit]))],
+                          uw: List[List[(String,
+  (List[Value.value], List[Value.value]))]],
+                          ux: List[(List[Nat.nat],
+                                     Transition.transition_ext[Unit])]):
+      Option[(List[AExp.aexp[VName.vname]],
+               List[(Nat.nat, AExp.aexp[VName.vname])])]
+  =
+  (x0, uu, uv, uw, ux) match {
+  case (Nil, uu, uv, uw, ux) => None
+  case (h :: t, p, e, l, g) =>
+    {
+      val updates:
+            FSet.fset[(List[Nat.nat],
+                        ((Nat.nat, Nat.nat), Transition.transition_ext[Unit]))]
+        = Lista.fold[(List[Nat.nat], Transition.transition_ext[Unit]),
+                      FSet.fset[(List[Nat.nat],
+                                  ((Nat.nat, Nat.nat),
+                                    Transition.transition_ext[Unit]))]](((a:
+                                    (List[Nat.nat],
+                                      Transition.transition_ext[Unit]))
+                                   =>
+                                  {
+                                    val (tids, ta):
+  (List[Nat.nat], Transition.transition_ext[Unit])
+                                      = a;
+                                    ((acc:
+FSet.fset[(List[Nat.nat],
+            ((Nat.nat, Nat.nat), Transition.transition_ext[Unit]))])
+                                       =>
+                                      replace_transition(acc, tids,
+                  Transition.Updates_update[Unit](((_:
+              List[(Nat.nat, AExp.aexp[VName.vname])])
+             =>
+            h),
+           ta)))
+                                  }),
+                                 g, e);
+      (find_outputs(p, updates, l,
+                     Lista.map[(List[Nat.nat], Transition.transition_ext[Unit]),
+                                (List[Nat.nat],
+                                  Transition.transition_ext[Unit])](((a:
+                                (List[Nat.nat],
+                                  Transition.transition_ext[Unit]))
+                               =>
+                              {
+                                val (id, ta):
+                                      (List[Nat.nat],
+Transition.transition_ext[Unit])
+                                  = a;
+                                (id, Transition.Updates_update[Unit](((_:
+                                 List[(Nat.nat, AExp.aexp[VName.vname])])
+                                =>
+                               h),
+                              ta))
+                              }),
+                             g))
+         match {
+         case None => find_updates_outputs(t, p, e, l, g)
+         case Some(pp) =>
+           Some[(List[AExp.aexp[VName.vname]],
+                  List[(Nat.nat, AExp.aexp[VName.vname])])]((pp, h))
+       })
+    }
+}
+
+def updates_same[A : HOL.equal, B, C](u1: (A, B), u2: (A, C)): Boolean =
+  HOL.eq[A](u1._1, u2._1)
+
+def standardise_group_outputs_updates(e:
+FSet.fset[(List[Nat.nat],
+            ((Nat.nat, Nat.nat), Transition.transition_ext[Unit]))],
+                                       l:
+ List[List[(String, (List[Value.value], List[Value.value]))]],
+                                       g:
+ List[(List[Nat.nat], Transition.transition_ext[Unit])]):
+      List[(List[Nat.nat], Transition.transition_ext[Unit])]
+  =
+  {
+    val update_groups: List[List[(Nat.nat, AExp.aexp[VName.vname])]] =
+      Lista.product_lists[(Nat.nat,
+                            AExp.aexp[VName.vname])](group_by[(Nat.nat,
+                        AExp.aexp[VName.vname])](((a:
+             (Nat.nat, AExp.aexp[VName.vname]))
+            =>
+           (b: (Nat.nat, AExp.aexp[VName.vname])) =>
+           updates_same[Nat.nat, AExp.aexp[VName.vname],
+                         AExp.aexp[VName.vname]](a, b)),
+          Lista.sort_key[(Nat.nat, AExp.aexp[VName.vname]),
+                          (Nat.nat,
+                            AExp.aexp[VName.vname])](((x:
+                 (Nat.nat, AExp.aexp[VName.vname]))
+                =>
+               x),
+              (Lista.maps[(List[Nat.nat], Transition.transition_ext[Unit]),
+                           (Nat.nat,
+                             AExp.aexp[VName.vname])](Fun.comp[Transition.transition_ext[Unit],
+                        List[(Nat.nat, AExp.aexp[VName.vname])],
+                        (List[Nat.nat],
+                          Transition.transition_ext[Unit])](((a:
+                        Transition.transition_ext[Unit])
+                       =>
+                      Transition.Updates[Unit](a)),
+                     ((a: (List[Nat.nat], Transition.transition_ext[Unit])) =>
+                       a._2)),
+               g)).par.distinct.toList)))
+    val update_groups_subs: List[List[(Nat.nat, AExp.aexp[VName.vname])]] =
+      Lista.fold[List[(Nat.nat, AExp.aexp[VName.vname])],
+                  List[List[(Nat.nat,
+                              AExp.aexp[VName.vname])]]](Fun.comp[List[List[(Nat.nat,
+                                      AExp.aexp[VName.vname])]],
+                           (List[List[(Nat.nat, AExp.aexp[VName.vname])]]) =>
+                             List[List[(Nat.nat, AExp.aexp[VName.vname])]],
+                           List[(Nat.nat,
+                                  AExp.aexp[VName.vname])]](Lista.union[List[(Nat.nat,
+                                       AExp.aexp[VName.vname])]],
+                     ((a: List[(Nat.nat, AExp.aexp[VName.vname])]) =>
+                       Lista.subseqs[(Nat.nat, AExp.aexp[VName.vname])](a))),
+                  update_groups, Nil)
+    val output_groups: List[List[AExp.aexp[VName.vname]]] =
+      Lista.product_lists[AExp.aexp[VName.vname]](Lista.transpose[AExp.aexp[VName.vname]]((Lista.map[(List[Nat.nat],
+                       Transition.transition_ext[Unit]),
+                      List[AExp.aexp[VName.vname]]](Fun.comp[Transition.transition_ext[Unit],
+                      List[AExp.aexp[VName.vname]],
+                      (List[Nat.nat],
+                        Transition.transition_ext[Unit])](((a:
+                      Transition.transition_ext[Unit])
+                     =>
+                    Transition.Outputs[Unit](a)),
+                   ((a: (List[Nat.nat], Transition.transition_ext[Unit])) =>
+                     a._2)),
+             g)).par.distinct.toList));
+    (find_updates_outputs(update_groups_subs, output_groups, e, l, g) match {
+       case None => g
+       case Some((p, u)) =>
+         Lista.map[(List[Nat.nat], Transition.transition_ext[Unit]),
+                    (List[Nat.nat],
+                      Transition.transition_ext[Unit])](((a:
+                    (List[Nat.nat], Transition.transition_ext[Unit]))
+                   =>
+                  {
+                    val (id, t):
+                          (List[Nat.nat], Transition.transition_ext[Unit])
+                      = a;
+                    (id, Transition.Updates_update[Unit](((_:
+                     List[(Nat.nat, AExp.aexp[VName.vname])])
+                    =>
+                   u),
+                  Transition.Outputs_update[Unit](((_:
+              List[AExp.aexp[VName.vname]])
+             =>
+            p),
+           t)))
+                  }),
+                 g)
+     })
+  }
+
 def trace_group_training_set(uu: List[(List[Nat.nat],
 Transition.transition_ext[Unit])],
                               uv: FSet.fset[(List[Nat.nat],
@@ -6625,11 +6854,11 @@ Transition.transition_ext[Unit])],
                               x4: List[(String,
  (List[Value.value], List[Value.value]))],
                               train:
-                                List[(Map[Nat.nat, Option[Value.value]],
-                                       (List[Value.value],
+                                List[(List[Value.value],
+                                       (Map[Nat.nat, Option[Value.value]],
  List[Value.value]))]):
-      List[(Map[Nat.nat, Option[Value.value]],
-             (List[Value.value], List[Value.value]))]
+      List[(List[Value.value],
+             (Map[Nat.nat, Option[Value.value]], List[Value.value]))]
   =
   (uu, uv, uw, ux, x4, train) match {
   case (uu, uv, uw, ux, Nil, train) => train
@@ -6655,7 +6884,7 @@ Transition.transition_ext[Unit])],
         trace_group_training_set(gp, e, sa,
                                   (Transition.apply_updates(Transition.Updates[Unit](transition),
                      AExp.join_ir(i, r))).apply(r),
-                                  t, (r, (i, p)) :: train)
+                                  t, (i, (r, p)) :: train)
         else trace_group_training_set(gp, e, sa,
                                        (Transition.apply_updates(Transition.Updates[Unit](transition),
                           AExp.join_ir(i, r))).apply(r),
@@ -6670,17 +6899,17 @@ def make_training_set(e: FSet.fset[(List[Nat.nat],
                                       (List[Value.value], List[Value.value]))]],
                        gp: List[(List[Nat.nat],
                                   Transition.transition_ext[Unit])]):
-      List[(Map[Nat.nat, Option[Value.value]],
-             (List[Value.value], List[Value.value]))]
+      List[(List[Value.value],
+             (Map[Nat.nat, Option[Value.value]], List[Value.value]))]
   =
   Lista.fold[List[(String, (List[Value.value], List[Value.value]))],
-              List[(Map[Nat.nat, Option[Value.value]],
-                     (List[Value.value],
+              List[(List[Value.value],
+                     (Map[Nat.nat, Option[Value.value]],
                        List[Value.value]))]](((a:
          List[(String, (List[Value.value], List[Value.value]))])
         =>
-       (b: List[(Map[Nat.nat, Option[Value.value]],
-                  (List[Value.value], List[Value.value]))])
+       (b: List[(List[Value.value],
+                  (Map[Nat.nat, Option[Value.value]], List[Value.value]))])
          =>
        trace_group_training_set(gp, e, Nat.zero_nata,
                                  scala.collection.immutable.Map().withDefaultValue(Option_ord.bot_option[Value.value]),
@@ -7609,52 +7838,14 @@ def generalise_and_update(log: List[List[(String,
     val values: List[Value.value] =
       Inference.enumerate_log_values_by_label(label, log)
     val new_gp_ts:
-          List[(Map[Nat.nat, Option[Value.value]],
-                 (List[Value.value], List[Value.value]))]
+          List[(List[Value.value],
+                 (Map[Nat.nat, Option[Value.value]], List[Value.value]))]
       = make_training_set(e, log, gp)
-    val i: List[List[Value.value]] =
-      Lista.map[(Map[Nat.nat, Option[Value.value]],
-                  (List[Value.value], List[Value.value])),
-                 List[Value.value]](((a:
-(Map[Nat.nat, Option[Value.value]], (List[Value.value], List[Value.value])))
-                                       =>
-                                      {
-val (_, (ins, _)):
-      (Map[Nat.nat, Option[Value.value]],
-        (List[Value.value], List[Value.value]))
-  = a;
-ins
-                                      }),
-                                     new_gp_ts)
-    val r: List[Map[Nat.nat, Option[Value.value]]] =
-      Lista.map[(Map[Nat.nat, Option[Value.value]],
-                  (List[Value.value], List[Value.value])),
-                 Map[Nat.nat, Option[Value.value]]](((a:
-                (Map[Nat.nat, Option[Value.value]],
-                  (List[Value.value], List[Value.value])))
-               =>
-              {
-                val (regs, (_, _)):
-                      (Map[Nat.nat, Option[Value.value]],
-                        (List[Value.value], List[Value.value]))
-                  = a;
-                regs
-              }),
-             new_gp_ts)
-    val p: List[List[Value.value]] =
-      Lista.map[(Map[Nat.nat, Option[Value.value]],
-                  (List[Value.value], List[Value.value])),
-                 List[Value.value]](((a:
-(Map[Nat.nat, Option[Value.value]], (List[Value.value], List[Value.value])))
-                                       =>
-                                      {
-val (_, (_, outs)):
-      (Map[Nat.nat, Option[Value.value]],
-        (List[Value.value], List[Value.value]))
-  = a;
-outs
-                                      }),
-                                     new_gp_ts)
+    val (i, (r, p)):
+          (List[List[Value.value]],
+            (List[Map[Nat.nat, Option[Value.value]]], List[List[Value.value]]))
+      = unzip_3[List[Value.value], Map[Nat.nat, Option[Value.value]],
+                 List[Value.value]](new_gp_ts)
     val max_reg: Nat.nat = Inference.max_reg_total(e)
     val outputs:
           List[Option[(AExp.aexp[VName.vname], Map[VName.vname, String])]]
@@ -7719,322 +7910,36 @@ outs
      })
   }
 
-def find_outputs(x0: List[List[AExp.aexp[VName.vname]]],
-                  uu: FSet.fset[(List[Nat.nat],
-                                  ((Nat.nat, Nat.nat),
-                                    Transition.transition_ext[Unit]))],
-                  uv: List[List[(String,
-                                  (List[Value.value], List[Value.value]))]],
-                  uw: List[(List[Nat.nat], Transition.transition_ext[Unit])]):
-      Option[List[AExp.aexp[VName.vname]]]
-  =
-  (x0, uu, uv, uw) match {
-  case (Nil, uu, uv, uw) => None
-  case (h :: t, e, l, g) =>
-    {
-      val outputs:
-            FSet.fset[(List[Nat.nat],
-                        ((Nat.nat, Nat.nat), Transition.transition_ext[Unit]))]
-        = Lista.fold[(List[Nat.nat], Transition.transition_ext[Unit]),
-                      FSet.fset[(List[Nat.nat],
-                                  ((Nat.nat, Nat.nat),
-                                    Transition.transition_ext[Unit]))]](((a:
-                                    (List[Nat.nat],
-                                      Transition.transition_ext[Unit]))
-                                   =>
-                                  {
-                                    val (tids, ta):
-  (List[Nat.nat], Transition.transition_ext[Unit])
-                                      = a;
-                                    ((acc:
-FSet.fset[(List[Nat.nat],
-            ((Nat.nat, Nat.nat), Transition.transition_ext[Unit]))])
-                                       =>
-                                      replace_transition(acc, tids,
-                  Transition.Outputs_update[Unit](((_:
-              List[AExp.aexp[VName.vname]])
-             =>
-            h),
-           ta)))
-                                  }),
-                                 g, e);
-      (if (Inference.satisfies(Set.seta[List[(String,
-       (List[Value.value], List[Value.value]))]](l),
-                                Inference.tm(outputs)))
-        Some[List[AExp.aexp[VName.vname]]](h) else find_outputs(t, e, l, g))
-    }
-}
-
-def find_updates_outputs(x0: List[List[(Nat.nat, AExp.aexp[VName.vname])]],
-                          uu: List[List[AExp.aexp[VName.vname]]],
-                          uv: FSet.fset[(List[Nat.nat],
-  ((Nat.nat, Nat.nat), Transition.transition_ext[Unit]))],
-                          uw: List[List[(String,
-  (List[Value.value], List[Value.value]))]],
-                          ux: List[(List[Nat.nat],
-                                     Transition.transition_ext[Unit])]):
-      Option[(List[AExp.aexp[VName.vname]],
-               List[(Nat.nat, AExp.aexp[VName.vname])])]
-  =
-  (x0, uu, uv, uw, ux) match {
-  case (Nil, uu, uv, uw, ux) => None
-  case (h :: t, p, e, l, g) =>
-    {
-      val updates:
-            FSet.fset[(List[Nat.nat],
-                        ((Nat.nat, Nat.nat), Transition.transition_ext[Unit]))]
-        = Lista.fold[(List[Nat.nat], Transition.transition_ext[Unit]),
-                      FSet.fset[(List[Nat.nat],
-                                  ((Nat.nat, Nat.nat),
-                                    Transition.transition_ext[Unit]))]](((a:
-                                    (List[Nat.nat],
-                                      Transition.transition_ext[Unit]))
-                                   =>
-                                  {
-                                    val (tids, ta):
-  (List[Nat.nat], Transition.transition_ext[Unit])
-                                      = a;
-                                    ((acc:
-FSet.fset[(List[Nat.nat],
-            ((Nat.nat, Nat.nat), Transition.transition_ext[Unit]))])
-                                       =>
-                                      replace_transition(acc, tids,
-                  Transition.Updates_update[Unit](((_:
-              List[(Nat.nat, AExp.aexp[VName.vname])])
-             =>
-            h),
-           ta)))
-                                  }),
-                                 g, e);
-      (find_outputs(p, updates, l,
-                     Lista.map[(List[Nat.nat], Transition.transition_ext[Unit]),
-                                (List[Nat.nat],
-                                  Transition.transition_ext[Unit])](((a:
-                                (List[Nat.nat],
-                                  Transition.transition_ext[Unit]))
-                               =>
-                              {
-                                val (id, ta):
-                                      (List[Nat.nat],
-Transition.transition_ext[Unit])
-                                  = a;
-                                (id, Transition.Updates_update[Unit](((_:
-                                 List[(Nat.nat, AExp.aexp[VName.vname])])
-                                =>
-                               h),
-                              ta))
-                              }),
-                             g))
-         match {
-         case None => find_updates_outputs(t, p, e, l, g)
-         case Some(pp) =>
-           Some[(List[AExp.aexp[VName.vname]],
-                  List[(Nat.nat, AExp.aexp[VName.vname])])]((pp, h))
-       })
-    }
-}
-
-def updates_same[A : HOL.equal, B, C](u1: (A, B), u2: (A, C)): Boolean =
-  HOL.eq[A](u1._1, u2._1)
-
-def power_list[A : HOL.equal : Orderings.linorder](l: List[A]): List[List[A]] =
-  Lista.sorted_list_of_set[List[A]](Set.image[Set.set[A],
-       List[A]](((a: Set.set[A]) => Lista.sorted_list_of_set[A](a)),
-                 Set.Pow[A](Set.seta[A](l))))
-
-def power_lists[A : HOL.equal : Orderings.linorder](l: List[List[A]]):
-      List[List[A]]
-  =
-  Lista.fold[List[A],
-              List[List[A]]](Fun.comp[List[List[A]],
-                                       (List[List[A]]) => List[List[A]],
-                                       List[A]](Lista.union[List[A]],
-         ((a: List[A]) => power_list[A](a))),
-                              l, Nil)
-
-def standardise_group_outputs_updates(e:
-FSet.fset[(List[Nat.nat],
-            ((Nat.nat, Nat.nat), Transition.transition_ext[Unit]))],
-                                       l:
- List[List[(String, (List[Value.value], List[Value.value]))]],
-                                       g:
- List[(List[Nat.nat], Transition.transition_ext[Unit])]):
-      List[(List[Nat.nat], Transition.transition_ext[Unit])]
+def standardise_group(e: FSet.fset[(List[Nat.nat],
+                                     ((Nat.nat, Nat.nat),
+                                       Transition.transition_ext[Unit]))],
+                       l: List[List[(String,
+                                      (List[Value.value], List[Value.value]))]],
+                       gp: List[(List[Nat.nat],
+                                  Transition.transition_ext[Unit])],
+                       s: (FSet.fset[(List[Nat.nat],
+                                       ((Nat.nat, Nat.nat),
+ Transition.transition_ext[Unit]))]) =>
+                            (List[List[(String,
+ (List[Value.value], List[Value.value]))]]) =>
+                              (List[(List[Nat.nat],
+                                      Transition.transition_ext[Unit])]) =>
+                                List[(List[Nat.nat],
+                                       Transition.transition_ext[Unit])]):
+      FSet.fset[(List[Nat.nat],
+                  ((Nat.nat, Nat.nat), Transition.transition_ext[Unit]))]
   =
   {
-    val update_groups: List[List[(Nat.nat, AExp.aexp[VName.vname])]] =
-      cartProdN[(Nat.nat,
-                  AExp.aexp[VName.vname])](group_by[(Nat.nat,
-              AExp.aexp[VName.vname])](((a: (Nat.nat, AExp.aexp[VName.vname]))
-  =>
- (b: (Nat.nat, AExp.aexp[VName.vname])) =>
- updates_same[Nat.nat, AExp.aexp[VName.vname], AExp.aexp[VName.vname]](a, b)),
-Lista.sort_key[(Nat.nat, AExp.aexp[VName.vname]),
-                (Nat.nat,
-                  AExp.aexp[VName.vname])](((x:
-       (Nat.nat, AExp.aexp[VName.vname]))
-      =>
-     x),
-    (Lista.maps[(List[Nat.nat], Transition.transition_ext[Unit]),
-                 (Nat.nat,
-                   AExp.aexp[VName.vname])](Fun.comp[Transition.transition_ext[Unit],
-              List[(Nat.nat, AExp.aexp[VName.vname])],
-              (List[Nat.nat],
-                Transition.transition_ext[Unit])](((a:
-              Transition.transition_ext[Unit])
-             =>
-            Transition.Updates[Unit](a)),
-           ((a: (List[Nat.nat], Transition.transition_ext[Unit])) => a._2)),
-     g)).par.distinct.toList)))
-    val update_groups_subs: List[List[(Nat.nat, AExp.aexp[VName.vname])]] =
-      power_lists[(Nat.nat, AExp.aexp[VName.vname])](update_groups)
-    val output_groups: List[List[AExp.aexp[VName.vname]]] =
-      cartProdN[AExp.aexp[VName.vname]](Lista.transpose[AExp.aexp[VName.vname]]((Lista.map[(List[Nat.nat],
-             Transition.transition_ext[Unit]),
-            List[AExp.aexp[VName.vname]]](Fun.comp[Transition.transition_ext[Unit],
-            List[AExp.aexp[VName.vname]],
-            (List[Nat.nat],
-              Transition.transition_ext[Unit])](((a:
-            Transition.transition_ext[Unit])
-           =>
-          Transition.Outputs[Unit](a)),
-         ((a: (List[Nat.nat], Transition.transition_ext[Unit])) => a._2)),
-   g)).par.distinct.toList));
-    (find_updates_outputs(update_groups_subs, output_groups, e, l, g) match {
-       case None => g
-       case Some((p, u)) =>
-         Lista.map[(List[Nat.nat], Transition.transition_ext[Unit]),
-                    (List[Nat.nat],
-                      Transition.transition_ext[Unit])](((a:
-                    (List[Nat.nat], Transition.transition_ext[Unit]))
-                   =>
-                  {
-                    val (id, t):
-                          (List[Nat.nat], Transition.transition_ext[Unit])
-                      = a;
-                    (id, Transition.Updates_update[Unit](((_:
-                     List[(Nat.nat, AExp.aexp[VName.vname])])
-                    =>
-                   u),
-                  Transition.Outputs_update[Unit](((_:
-              List[AExp.aexp[VName.vname]])
-             =>
-            p),
-           t)))
-                  }),
-                 g)
-     })
+    val standardised: List[(List[Nat.nat], Transition.transition_ext[Unit])] =
+      ((s(e))(l))(gp)
+    val ea: FSet.fset[(List[Nat.nat],
+                        ((Nat.nat, Nat.nat), Transition.transition_ext[Unit]))]
+      = Inference.replace_transitions(e, standardised);
+    (if (Inference.satisfies(Set.seta[List[(String,
+     (List[Value.value], List[Value.value]))]](l),
+                              Inference.tm(ea)))
+      ea else e)
   }
-
-def standardise_groups_aux(e: FSet.fset[(List[Nat.nat],
-  ((Nat.nat, Nat.nat), Transition.transition_ext[Unit]))],
-                            l: List[List[(String,
-   (List[Value.value], List[Value.value]))]],
-                            xs: List[List[(List[Nat.nat],
-    Transition.transition_ext[Unit])]],
-                            s: (FSet.fset[(List[Nat.nat],
-    ((Nat.nat, Nat.nat), Transition.transition_ext[Unit]))]) =>
-                                 (List[List[(String,
-      (List[Value.value], List[Value.value]))]]) =>
-                                   (List[(List[Nat.nat],
-   Transition.transition_ext[Unit])]) =>
-                                     List[(List[Nat.nat],
-    Transition.transition_ext[Unit])]):
-      FSet.fset[(List[Nat.nat],
-                  ((Nat.nat, Nat.nat), Transition.transition_ext[Unit]))]
-  =
-  Lista.fold[List[(List[Nat.nat], Transition.transition_ext[Unit])],
-              FSet.fset[(List[Nat.nat],
-                          ((Nat.nat, Nat.nat),
-                            Transition.transition_ext[Unit]))]](((h:
-                            List[(List[Nat.nat],
-                                   Transition.transition_ext[Unit])])
-                           =>
-                          (acc: FSet.fset[(List[Nat.nat],
-    ((Nat.nat, Nat.nat), Transition.transition_ext[Unit]))])
-                            =>
-                          {
-                            val ea: FSet.fset[(List[Nat.nat],
-        ((Nat.nat, Nat.nat), Transition.transition_ext[Unit]))]
-                              = Inference.replace_transitions(acc,
-                       ((s(acc))(l))(h));
-                            (if (Inference.satisfies(Set.seta[List[(String,
-                             (List[Value.value], List[Value.value]))]](l),
-              Inference.tm(ea)))
-                              ea else acc)
-                          }),
-                         xs, e)
-
-def group_by_structure(e: FSet.fset[(List[Nat.nat],
-                                      ((Nat.nat, Nat.nat),
-Transition.transition_ext[Unit]))]):
-      List[List[(List[Nat.nat], Transition.transition_ext[Unit])]]
-  =
-  Lista.map[List[(Transition.transition_ext[Unit], List[Nat.nat])],
-             List[(List[Nat.nat],
-                    Transition.transition_ext[Unit])]](((a:
-                   List[(Transition.transition_ext[Unit], List[Nat.nat])])
-                  =>
-                 Lista.map[(Transition.transition_ext[Unit], List[Nat.nat]),
-                            (List[Nat.nat],
-                              Transition.transition_ext[Unit])](((aa:
-                            (Transition.transition_ext[Unit], List[Nat.nat]))
-                           =>
-                          {
-                            val (t, id):
-                                  (Transition.transition_ext[Unit],
-                                    List[Nat.nat])
-                              = aa;
-                            (id, t)
-                          }),
-                         a)),
-                group_by[(Transition.transition_ext[Unit],
-                           List[Nat.nat])](((a:
-       (Transition.transition_ext[Unit], List[Nat.nat]))
-      =>
-     {
-       val (t1, _): (Transition.transition_ext[Unit], List[Nat.nat]) = a;
-       ((aa: (Transition.transition_ext[Unit], List[Nat.nat])) =>
-         {
-           val (t2, _): (Transition.transition_ext[Unit], List[Nat.nat]) = aa;
-           Transition.same_structure(t1, t2)
-         })
-     }),
-    FSet.sorted_list_of_fset[(Transition.transition_ext[Unit],
-                               List[Nat.nat])](FSet.fimage[(List[Nat.nat],
-                     ((Nat.nat, Nat.nat), Transition.transition_ext[Unit])),
-                    (Transition.transition_ext[Unit],
-                      List[Nat.nat])](((a:
-  (List[Nat.nat], ((Nat.nat, Nat.nat), Transition.transition_ext[Unit])))
- =>
-{
-  val (id, (_, t)):
-        (List[Nat.nat], ((Nat.nat, Nat.nat), Transition.transition_ext[Unit]))
-    = a;
-  (t, id)
-}),
-                                       e))))
-
-def standardise_groups(e: FSet.fset[(List[Nat.nat],
-                                      ((Nat.nat, Nat.nat),
-Transition.transition_ext[Unit]))],
-                        l: List[List[(String,
-                                       (List[Value.value],
- List[Value.value]))]]):
-      FSet.fset[(List[Nat.nat],
-                  ((Nat.nat, Nat.nat), Transition.transition_ext[Unit]))]
-  =
-  standardise_groups_aux(e, l, group_by_structure(e),
-                          ((a: FSet.fset[(List[Nat.nat],
-   ((Nat.nat, Nat.nat), Transition.transition_ext[Unit]))])
-                             =>
-                            (b: List[List[(String,
-    (List[Value.value], List[Value.value]))]])
-                              =>
-                            (c: List[(List[Nat.nat],
-                                       Transition.transition_ext[Unit])])
-                              =>
-                            standardise_group_outputs_updates(a, b, c)))
 
 def merge_if_same(e: FSet.fset[(List[Nat.nat],
                                  ((Nat.nat, Nat.nat),
@@ -8150,11 +8055,60 @@ def groupwise_generalise_and_update(uu: List[List[(String,
        case None => groupwise_generalise_and_update(log, e, t)
        case Some(ea) =>
          {
+           val rep: Transition.transition_ext[Unit] = (gp.head)._2
+           val structural_group:
+                 FSet.fset[(List[Nat.nat], Transition.transition_ext[Unit])]
+             = FSet.fimage[(List[Nat.nat],
+                             ((Nat.nat, Nat.nat),
+                               Transition.transition_ext[Unit])),
+                            (List[Nat.nat],
+                              Transition.transition_ext[Unit])](((a:
+                            (List[Nat.nat],
+                              ((Nat.nat, Nat.nat),
+                                Transition.transition_ext[Unit])))
+                           =>
+                          {
+                            val (id, aa):
+                                  (List[Nat.nat],
+                                    ((Nat.nat, Nat.nat),
+                                      Transition.transition_ext[Unit]))
+                              = a
+                            val (_, ab):
+                                  ((Nat.nat, Nat.nat),
+                                    Transition.transition_ext[Unit])
+                              = aa;
+                            (id, ab)
+                          }),
+                         FSet.ffilter[(List[Nat.nat],
+((Nat.nat, Nat.nat),
+  Transition.transition_ext[Unit]))](((a:
+ (List[Nat.nat], ((Nat.nat, Nat.nat), Transition.transition_ext[Unit])))
+=>
+                                       {
+ val (_, (_, ta)):
+       (List[Nat.nat], ((Nat.nat, Nat.nat), Transition.transition_ext[Unit]))
+   = a;
+ Transition.same_structure(ta, rep)
+                                       }),
+                                      ea))
            val standardised:
                  FSet.fset[(List[Nat.nat],
                              ((Nat.nat, Nat.nat),
                                Transition.transition_ext[Unit]))]
-             = standardise_groups(ea, log);
+             = standardise_group(e, log,
+                                  FSet.sorted_list_of_fset[(List[Nat.nat],
+                     Transition.transition_ext[Unit])](structural_group),
+                                  ((a: FSet.fset[(List[Nat.nat],
+           ((Nat.nat, Nat.nat), Transition.transition_ext[Unit]))])
+                                     =>
+                                    (b: List[List[(String,
+            (List[Value.value], List[Value.value]))]])
+                                      =>
+                                    (c: List[(List[Nat.nat],
+       Transition.transition_ext[Unit])])
+                                      =>
+                                    standardise_group_outputs_updates(a, b,
+                               c)));
            groupwise_generalise_and_update(log, merge_regs(standardised, log),
     t)
          }
@@ -8503,13 +8457,8 @@ List[Nat.nat]))))]):
                                 delay_initialisation_of(r, log, acc,
                  find_first_uses_of(r, log, acc))),
                                Lista.sorted_list_of_set[Nat.nat](Inference.all_regs(normalised)),
-                               normalised)
-    val merged:
-          FSet.fset[(List[Nat.nat],
-                      ((Nat.nat, Nat.nat), Transition.transition_ext[Unit]))]
-      = merge_regs(delayed, log);
-    standardise_groups(merged, log);
-    drop_all_guards(merged, pta, log, m, np)
+                               normalised);
+    drop_all_guards(delayed, pta, log, m, np)
   }
 
 def drop_pta_guards(pta: FSet.fset[(List[Nat.nat],
